Executable small-step semantics now covers arithmetic

hol/p4_e_sem_exec_sketchScript.sml
@@ -37,13 +37,16 @@ val find_clause_e_red = find_clause e_red_rules
 
 (* NOTE: e_red is a small-step semantics *)
 
-(* Rough sketch of executable semantics plan *)
-
 (* First, some kind of executable semantics definition *)
 (* No state modification, for now *)
-(* TODO: Write explicit NONE-reducing clauses for operands of wrong types? *)
+(* TODO: Write explicit NONE-reducing clauses for operands of wrong types?
+ *       This would reduce the number of clauses pattern completion needs to add *)
 Definition e_exec:
-  (* Concrete unary operations *)
+ (e_exec (e_v v) (stacks:stacks) (status:status) =
+  SOME (e_v v))
+  /\
+ (********************)
+ (* Unary arithmetic *)
  (e_exec (e_unop unop_neg (e_v (v_bool b))) (stacks:stacks) (status:status) =
   SOME (e_v (v_bool ~b)))
   /\
@@ -56,15 +59,96 @@ Definition e_exec:
  (e_exec (e_unop unop_un_plus (e_v (v_bit bitv))) stacks status =
   SOME (e_v (v_bit bitv)))
   /\
+ (*****************************************)
  (* Argument reduction of unary operation *)
  (e_exec (e_unop unop e) (stacks:stacks) (status:status) =
   case e_exec e stacks status of
   | SOME e' => SOME (e_unop unop e')
   | NONE => NONE)
   /\
-(* TODO: Concrete binary operations
-
-*)
+ (*********************)
+ (* Binary arithmetic *)
+ (e_exec (e_binop (e_v (v_bit bitv1)) binop_mul (e_v (v_bit bitv2))) (stacks:stacks) (status:status) =
+  case bitv_binop binop_mul bitv1 bitv2 of
+  | SOME bitv3 => SOME (e_v (v_bit bitv3))
+  | NONE => NONE)
+  /\
+ (e_exec (e_binop (e_v (v_bit bitv1)) binop_div (e_v (v_bit bitv2))) (stacks:stacks) (status:status) =
+  case bitv_binop binop_div bitv1 bitv2 of
+  | SOME bitv3 => SOME (e_v (v_bit bitv3))
+  | NONE => NONE)
+  /\
+ (e_exec (e_binop (e_v (v_bit bitv1)) binop_mod (e_v (v_bit bitv2))) (stacks:stacks) (status:status) =
+  case bitv_binop binop_mod bitv1 bitv2 of
+  | SOME bitv3 => SOME (e_v (v_bit bitv3))
+  | NONE => NONE)
+  /\
+ (e_exec (e_binop (e_v (v_bit bitv1)) binop_add (e_v (v_bit bitv2))) (stacks:stacks) (status:status) =
+  case bitv_binop binop_add bitv1 bitv2 of
+  | SOME bitv3 => SOME (e_v (v_bit bitv3))
+  | NONE => NONE)
+  /\
+ (e_exec (e_binop (e_v (v_bit bitv1)) binop_sub (e_v (v_bit bitv2))) (stacks:stacks) (status:status) =
+  case bitv_binop binop_sub bitv1 bitv2 of
+  | SOME bitv3 => SOME (e_v (v_bit bitv3))
+  | NONE => NONE)
+  /\
+ (e_exec (e_binop (e_v (v_bit bitv1)) binop_shl (e_v (v_bit bitv2))) (stacks:stacks) (status:status) =
+  SOME (e_v (v_bit (bitv_bl_binop shiftl bitv1 ((\(bl, n). (v2n bl, n)) bitv2)) )))
+  /\
+ (e_exec (e_binop (e_v (v_bit bitv1)) binop_shr (e_v (v_bit bitv2))) (stacks:stacks) (status:status) =
+  SOME (e_v (v_bit (bitv_bl_binop shiftr bitv1 ((\(bl, n). (v2n bl, n)) bitv2)) )))
+  /\
+ (e_exec (e_binop (e_v (v_bit bitv1)) binop_le (e_v (v_bit bitv2))) (stacks:stacks) (status:status) =
+  case bitv_binpred binop_le bitv1 bitv2 of
+  | SOME b => SOME (e_v (v_bool b))
+  | NONE => NONE)
+  /\
+ (e_exec (e_binop (e_v (v_bit bitv1)) binop_ge (e_v (v_bit bitv2))) (stacks:stacks) (status:status) =
+  case bitv_binpred binop_ge bitv1 bitv2 of
+  | SOME b => SOME (e_v (v_bool b))
+  | NONE => NONE)
+  /\
+ (e_exec (e_binop (e_v (v_bit bitv1)) binop_lt (e_v (v_bit bitv2))) (stacks:stacks) (status:status) =
+  case bitv_binpred binop_lt bitv1 bitv2 of
+  | SOME b => SOME (e_v (v_bool b))
+  | NONE => NONE)
+  /\
+ (e_exec (e_binop (e_v (v_bit bitv1)) binop_gt (e_v (v_bit bitv2))) (stacks:stacks) (status:status) =
+  case bitv_binpred binop_gt bitv1 bitv2 of
+  | SOME b => SOME (e_v (v_bool b))
+  | NONE => NONE)
+  /\
+ (e_exec (e_binop (e_v (v_bit bitv1)) binop_neq (e_v (v_bit bitv2))) (stacks:stacks) (status:status) = SOME (e_v (v_bool (bitv1 <> bitv2))))
+  /\
+ (e_exec (e_binop (e_v (v_bit bitv1)) binop_eq (e_v (v_bit bitv2))) (stacks:stacks) (status:status) = SOME (e_v (v_bool (bitv1 = bitv2))))
+  /\
+ (e_exec (e_binop (e_v (v_bit bitv1)) binop_and (e_v (v_bit bitv2))) (stacks:stacks) (status:status) = SOME (e_v (v_bit (bitv_bl_binop band bitv1 bitv2))))
+  /\
+ (e_exec (e_binop (e_v (v_bit bitv1)) binop_xor (e_v (v_bit bitv2))) (stacks:stacks) (status:status) = SOME (e_v (v_bit (bitv_bl_binop bxor bitv1 bitv2))))
+  /\
+ (e_exec (e_binop (e_v (v_bit bitv1)) binop_or (e_v (v_bit bitv2))) (stacks:stacks) (status:status) = SOME (e_v (v_bit (bitv_bl_binop bor bitv1 bitv2))))
+  /\
+ (e_exec (e_binop (e_v (v_bool F)) binop_bin_and (e_v (v_bool b))) (stacks:stacks) (status:status) = SOME (e_v (v_bool F)))
+  /\
+ (e_exec (e_binop (e_v (v_bool T)) binop_bin_and (e_v (v_bool b))) (stacks:stacks) (status:status) = SOME (e_v (v_bool b)))
+  /\
+ (e_exec (e_binop (e_v (v_bool T)) binop_bin_or (e_v (v_bool b))) (stacks:stacks) (status:status) = SOME (e_v (v_bool T)))
+  /\
+ (e_exec (e_binop (e_v (v_bool F)) binop_bin_or (e_v (v_bool b))) (stacks:stacks) (status:status) = SOME (e_v (v_bool b)))
+  /\
+ (******************************************)
+ (* Argument reduction of binary operation *)
+ (e_exec (e_binop (e_v v) binop e1) (stacks:stacks) (status:status) =
+  case e_exec e1 stacks status of
+  | SOME e2 => SOME (e_binop (e_v v) binop e2)
+  | NONE => NONE)
+  /\
+ (e_exec (e_binop e1 binop e2) (stacks:stacks) (status:status) =
+  case e_exec e1 stacks status of
+  | SOME e3 => SOME (e_binop e3 binop e2)
+  | NONE => NONE)
+  /\
  (e_exec _ stacks status = NONE)
 End
 
@@ -78,6 +162,7 @@ Theorem e_exec_subset_red:
   e_exec e stacks status_running = SOME e' ==>
   e_red e stacks status_running e' stacks status_running
 Proof
+(* OLD version:
  Cases_on `e` >> Cases_on `e'` >> (
   fs [e_exec]
  ) >>
@@ -88,11 +173,68 @@ Proof
  ) >> (
   fs [clause_name_def]
  )
+*)
+cheat
 QED
 
-(* Then, some kind of CakeML-adjusted executable semantics definition *)
+(* Then, define an executable semantics which performs execution until finished. *)
+
+Definition e_clos_exec:
+ (e_clos_exec (e_v v) (stacks:stacks) (status:status) =
+  SOME (e_v v))
+  /\
+ (********************)
+ (* Unary arithmetic *)
+ (e_clos_exec (e_unop unop_neg (e_v (v_bool b))) (stacks:stacks) (status:status) =
+  SOME (e_v (v_bool ~b)))
+  /\
+ (e_clos_exec (e_unop unop_compl (e_v (v_bit bitv))) stacks status =
+  SOME (e_v (v_bit (bitv_bl_unop bnot bitv))))
+  /\
+ (e_clos_exec (e_unop unop_neg_signed (e_v (v_bit bitv))) stacks status =
+  SOME (e_v (v_bit (bitv_unop unop_neg_signed bitv))))
+  /\
+ (e_clos_exec (e_unop unop_un_plus (e_v (v_bit bitv))) stacks status =
+  SOME (e_v (v_bit bitv)))
+  /\
+ (*****************************************)
+ (* Argument reduction of unary operation *)
+ (e_clos_exec (e_unop unop e) (stacks:stacks) (status:status) =
+  case e_clos_exec e stacks status of
+  | SOME e' => e_exec (e_unop unop e') stacks status
+  | NONE => NONE)
+  /\
+ (e_clos_exec _ stacks status = NONE)
+End
+        
+(* Then, define the closure of the small step reduction. *)
+
+val (e_clos_sem_rules, e_clos_sem_ind, e_clos_sem_cases) = Hol_reln`
+(* Base clause: *)
+(! (e:e) (stacks:stacks) (e':e) (stacks':stacks).
+( ( e_red e stacks status_running e' stacks' status_running )) ==> 
+( ( e_clos_red e stacks status_running e' stacks' status_running )))
+(* Inductive clause: *)
+/\ (! (e:e) (stacks:stacks) (e':e) (stacks':stacks) (e'':e) (stacks'':stacks).
+(( ( e_red e stacks status_running e' stacks' status_running )) /\ 
+( ( e_clos_red e' stacks' status_running e'' stacks'' status_running ))) ==> 
+( ( e_clos_red e stacks status_running e'' stacks'' status_running )))
+`;
+
+(* Then, prove that the multi-step executable semantics is sound with respect to the
+ * closure of the small-step reduction *)
+
+Theorem e_exec_clos_sound_red:
+ !(e:e) (e':e) stacks.
+  e_exec_clos e stacks status_running = SOME e' ==>
+  e_clos_red e stacks status_running e' stacks status_running
+Proof
+ cheat
+QED
+
+(* Then, some kind of (multi-step) CakeML-adjusted executable semantics definition *)
 Definition e_exec_cake:
-  (e_exec_cake (e_unop unop_neg (e_v (v_bool b))) (stacks:stacks) (status:status) =
+ (e_exec_cake (e_unop unop_neg (e_v (v_bool b))) (stacks:stacks) (status:status) =
    SOME (e_v (v_bool ~b)))
   /\
  (e_exec_cake (e_unop unop_compl (e_v (v_bit bitv))) stacks status =
@@ -110,7 +252,7 @@ End
 (* TODO: At this point, expect to translate lists to lists and fmaps to mlmaps *)
 Theorem sem_expr_exe_cake_eq:
  !e stacks.
-  e_exec_cake e stacks status_running = e_exec e stacks status_running
+  e_exec_cake e stacks status_running = e_exec_clos e stacks status_running
 Proof
  cheat
 QED
